Work on termination for pattern compile
Some effort on proving structural results, but focus on termination for now
Previous metric not enough - need exponents for OR patterns
Proved first result (dispatch), which is hard one - prove rest

proofs/core/Pattern.v
@@ -86,10 +86,12 @@ Fixpoint simplify_aux (a: A) (p: pattern) : list (pattern * A) :=
   end.
 
 Definition simplify_single (x: list pattern * A) : list (list pattern * A) :=
-  let (ps, a) := x in
-  let p := List.hd Pwild ps in
-    let ptl := List.tl ps in
-    map (fun '(p1, y) => (p1 :: ptl, y)) (simplify_aux a p).
+    let (ps, a) := x in
+    match ps with
+    | p :: ptl => 
+      map (fun '(p1, y) => (p1 :: ptl, y)) (simplify_aux a p)
+    | nil => nil
+    end.
 
 Definition simplify (rl: list (list pattern * A)) : list (list pattern * A) :=
   concat (map simplify_single rl).
@@ -107,9 +109,12 @@ Definition dispatch2_aux (x: list pattern * A)
   | _ => (*impossible*) (cases, wilds)
   end.
 
-Definition dispatch2 (rl: list (list pattern * A)) :
+Definition dispatch2_gen (rl: list (list pattern * A)) :
   amap funsym (list (list pattern * A)) * list (list pattern * A) :=
-  fold_right dispatch2_aux (amap_empty, nil) (simplify rl).
+  fold_right dispatch2_aux (amap_empty, nil) rl.
+
+Definition dispatch2 (rl: list (list pattern * A)) :=
+  dispatch2_gen (simplify rl).
 
 (*We need this for the odd induction principle*)
 Lemma dispatch_equiv_aux x base 
@@ -131,7 +136,7 @@ Qed.
 Lemma dispatch_equiv rl (Hrl: Forall (fun x => negb (null (fst x))) rl):
   dispatch1 rl = dispatch2 rl.
 Proof.
-  unfold dispatch2, dispatch1.
+  unfold dispatch2, dispatch2_gen, dispatch1.
   induction rl as [|[pl a] ps IH]; simpl; auto.
   inversion Hrl as [|? ? Hpl Hps]; subst; simpl in *.
   unfold simplify in *. simpl.
@@ -177,33 +182,9 @@ Definition term_list_size (l: list term) : nat :=
 Definition compile_size (l: list (list pattern * A)) : nat :=
   sum (map pat_list_size (map fst l)).
 
-(*NOTE: will try to do with pattern, I think that is terminating*)
-Equations compile (tl: list (term * vty)) (rl: list (list pattern * A)) : option A 
-  by wf (compile_size rl) lt :=
-  compile _ [] := None;
-  compile [] ((_, a) :: _) => Some a;
-  compile ((t, ty) :: tl) rl =>
-  (* match tl, rl with
-  | _, [] => None
-  | nil, (_, a) :: _ => Some a
-  | (t, ty) :: tl, _ => *)
-    (*No bare*)
-    (*extarct the set of constructors*)
-    let css :=
-    match ty with
-    | vty_cons ts _ => get_constructors ts
-    | _ => nil
-    end in
-    (*NOTE: no metadata in funsym saying constructor*)
-    let is_constr fs := in_bool funsym_eq_dec fs css in
-
-    (*Here, we do the simplify/dispatch*)
-
-    (*Map every constructor ocurring at the head of the pattern list to the
-      list of its args*)
-    let (types, cslist) :=
-      (*NOTE: we don't have maps, not ideal*)
-      let fix populate (acc : amap funsym (list pattern) * list (funsym * list vty * list pattern)) 
+Section Populate.
+Variable (is_constr : funsym -> bool).
+Fixpoint populate  (acc : amap funsym (list pattern) * list (funsym * list vty * list pattern)) 
         (p: pattern) : amap funsym (list pattern) * list (funsym * list vty * list pattern) :=
         match p with
         | Pwild => acc
@@ -216,28 +197,513 @@ Equations compile (tl: list (term * vty)) (rl: list (list pattern * A)) : option
           else acc (*impossible case - Why3 throws exception here*)
         | Por p1 p2 => populate (populate acc p1) p2
         | Pbind p _ => populate acc p
-        end
-      in
-      fold_left populate (map (fun x => List.hd Pwild (fst x)) rl) (amap_empty, nil) 
+        end.
+End Populate.
+
+(*Before we can define the full function, we need proofs for termination.
+  These proofs will be very useful for correctness later on.
+  First, the key property characterizing the results of dispatch in a clear, functional way*)
+Check dispatch1.
+Check amap_mem.
+
+Definition is_pat_constr (cs: funsym) (p: pattern) : option (list vty * list pattern) :=
+  match p with
+  | Pconstr f tys ps => if funsym_eqb cs f then Some (tys, ps) else None
+  | _ => None
+end.
+Check repeat.
+(*assume that we have already simplified the pattern match, so it only has constructors and wilds*)
+(*NOTE: need to know that all instances of Pconstr f ps for same f has ps with same length (implied by typing)*)
+Check dispatch2.
+(*TODO: define map_filter operation: filter, then map*)
+Definition filter_map {A B: Type} (f: A -> option B) (l: list A): list B :=
+  fold_right (fun x acc => match (f x) with | None => acc | Some y => y :: acc end) nil l.
+Check amap_get.
+
+Definition populate_all (is_constr: funsym -> bool) (rl: list (list pattern * A)) :=
+  fold_left (populate is_constr) (map (fun x => List.hd Pwild (fst x)) rl) (amap_empty, nil).
+Check populate_all.
+
+Definition pat_at_head (p: pattern) (r: list pattern * A) : bool :=
+  match (fst r) with | p1 :: _ => pattern_eqb p p1 | _ => false end.
+Definition constr_at_head (c: funsym) (r: list pattern * A) : bool :=
+  match (fst r) with | Pconstr f _ _ :: _ => funsym_eqb f c | _ => false end.
+
+(*list has every (cs, tys, ps) tuple that is the first ocurrence of cs*)
+(*An easier, but much less efficient definition*)
+Definition find_last {A: Type} (p: A -> bool) (l: list A) : option A :=
+  fold_right (fun x acc => match acc with | Some y => Some y | None => if p x then Some x else None end) None l.
+
+Lemma find_app1 {B: Type} (p: B -> bool) (l1 l2: list B) x:
+  find p l1 = Some x ->
+  find p (l1 ++ l2) = Some x.
+Proof.
+  induction l1 as [|h t IH]; simpl; try discriminate.
+  destruct (p h); auto.
+Qed.
+
+Lemma find_app2 {B: Type} (p: B -> bool) (l1 l2: list B):
+  find p l1 = None ->
+  find p (l1 ++ l2) = find p l2.
+Proof.
+  induction l1 as [|h t IH]; simpl; auto.
+  destruct (p h); auto. discriminate.
+Qed.
+
+Lemma find_app3 {B: Type} (p: B -> bool) (l1 l2: list B):
+  find p l2 = None ->
+  find p (l1 ++ l2) = find p l1.
+Proof.
+  induction l1 as [|h t IH]; simpl; auto.
+  destruct (p h); auto.
+Qed.
+
+Lemma find_rev {B: Type} (p: B -> bool) (l: list B):
+  find p (rev l) = find_last p l.
+Proof.
+  induction l; simpl; auto.
+  destruct (find_last p l).
+  - apply find_app1. auto.
+  - rewrite find_app2; auto.
+Qed. 
+
+(*Prove map, prove list has same things as map, don't care about order here I think? - maybe just
+  prove bindings*)
+(*NOTE: we can assume that rl is simplified (TODO change in compile)*)
+(*Incorrect: store funsym + list pattern in that pattern*)
+
+(*TODO: maybe prove after, almost proved, first focus on termination, which must be unconditional*)
+(*
+Lemma populate_all_types_constr (is_constr: funsym -> bool) rl cs (Hconstr: is_constr cs)
+  (Hrl: Forall (fun x => negb (null (fst x))) rl):
+  amap_get funsym_eq_dec (fst (populate_all is_constr rl)) cs =
+  option_map fst (find (constr_at_head cs) rl).
+Proof.
+  unfold populate_all.
+  rewrite <- fold_left_rev_right, <- map_rev.
+  rewrite <- (rev_involutive rl) at 2. (*TODO: maybe don't need [find_rev]*)
+  apply Forall_rev in Hrl.
+  induction (rev rl) as [| [ps a] t IH]; simpl.
+  - rewrite amap_empty_get. reflexivity.
+  - inversion Hrl as [|? ? Hnull Hrl']; subst; simpl in *. 
+    destruct ps as [|phd ptl]; try discriminate.
+    simpl. destruct phd as [v|f tys pats| | | ]; simpl; try solve[rewrite IH; auto; rewrite find_app3; auto].
+    + (*Pconstr*)
+      destruct (fold_right
+          (fun (y : pattern) (x : amap funsym (list pattern) * list (funsym * list vty * list pattern))
+           => populate is_constr x y) (amap_empty, [])
+          (map (fun x : list pattern * A => hd Pwild (fst x)) t)) as [css csl].
+      simpl in IH. specialize (IH Hrl').
+      destruct (funsym_eqb_spec f cs).
+      * subst. rewrite Hconstr.
+        rewrite amap_mem_spec, IH.
+        destruct (find (constr_at_head cs) (rev t)) as [x|] eqn : Hfind; simpl.
+        -- rewrite find_app1 with (x:=x); auto.
+        -- rewrite find_app2; auto. simpl.
+           unfold constr_at_head. simpl. destruct (funsym_eqb_spec cs cs); auto; try contradiction.
+           simpl. rewrite amap_set_get_same. Search amap_get amap_set.
+        *)
+  
+
+(*TODO: do we need to know that only Pwild/Pconstr*)
+
+(*First, let's prove something about [types] and [cslist] - should be easier*)
+(*Probably need map equivalence*)
+
+
+
+(*Lemma dispatch2_gen_fst (types: amap funsym (list pattern)) rl cs args
+  (*Cannot be iff for IH*)
+  (*(Htypes: forall cs args, amap_get funsym_eq_dec types cs = Some args ->
+    exists ps tys a, In (Pconstr cs tys args :: ps, a) rl)*):
+  amap_get funsym_eq_dec types cs = Some args ->
+  amap_get funsym_eq_dec (fst (dispatch2_gen types rl)) cs = Some
+    (filter_map (fun x =>
+    let ps := fst x in
+    let a := snd x in
+    let p := hd Pwild ps in
+    let ps := tl ps in
+    match p with
+    | Pwild => Some (repeat Pwild (length args) ++ ps, a)
+    | Pconstr fs tys pats =>
+        if funsym_eqb fs cs then Some (rev pats ++ ps, a) else None
+    | _ => None
+    end) rl).
+Proof.
+  intros Htypesget.
+  induction rl as [| [ps a] rtl IH]; simpl.
+  - apply Htypes in Htypesget. destruct_all; contradiction.
+  - simpl in Htypes. rewrite amap_empty_get. in Hget. discriminate.
+  - destruct (dispatch2_gen types rtl) as [cases wilds] eqn : Hrec.
+    simpl in *. 
+
+
+  (*(rl_wf: forall c tys1 tys2 ps1 ps2 l1 l2, In (Pconstr c tys1 ps1) (concat (map fst l1)) -> 
+    In (Pconstr c tys2 ps2) (concat (map fst l2)) -> length tys1 = length tys2 /\ length ps1 = length ps2):*):
+  amap_get funsym_eq_dec (fst (dispatch2_gen types rl)) cs = Some l ->
+  l = filter_map (fun x =>
+    let ps := fst x in
+    let a := snd x in
+    let p := hd Pwild ps in
+    let ps := tl ps in
+    match (amap_get funsym_eq_dec types cs) with
+    | None => (*impossible*) None
+    | Some args =>
+        match p with
+        | Pwild => Some (repeat Pwild (length args) ++ ps, a)
+        | Pconstr fs tys pats =>
+            if funsym_eqb fs cs then Some (rev pats ++ ps, a) else None
+        | _ => None
+        end 
+    end) rl.
+Proof.
+
+
+Lemma dispatch2_gen_fst (types: amap funsym (list pattern)) rl cs l
+
+
+  (*(rl_wf: forall c tys1 tys2 ps1 ps2 l1 l2, In (Pconstr c tys1 ps1) (concat (map fst l1)) -> 
+    In (Pconstr c tys2 ps2) (concat (map fst l2)) -> length tys1 = length tys2 /\ length ps1 = length ps2):*):
+  amap_get funsym_eq_dec (fst (dispatch2_gen types rl)) cs = Some l ->
+  l = filter_map (fun x =>
+    let ps := fst x in
+    let a := snd x in
+    let p := hd Pwild ps in
+    let ps := tl ps in
+    match (amap_get funsym_eq_dec types cs) with
+    | None => (*impossible*) None
+    | Some args =>
+        match p with
+        | Pwild => Some (repeat Pwild (length args) ++ ps, a)
+        | Pconstr fs tys pats =>
+            if funsym_eqb fs cs then Some (rev pats ++ ps, a) else None
+        | _ => None
+        end 
+    end) rl.
+Proof.
+  induction rl as [| [ps a] rtl IH]; simpl.
+  - intros Hget. rewrite amap_empty_get in Hget. discriminate.
+  - destruct (dispatch2_gen types rtl) as [cases wilds] eqn : Hrec.
+    simpl in *. 
+ discrimintae. Search amap_empty.
+
+Proof.
+  
+
+
+  
+  l = map (filter (fun x =>
+    let ps := fst x in
+    let a := snd x in
+  rl).
+  *)
+Print compile_size.
+Lemma compile_size_cons p l:
+  compile_size (p :: l) = pat_list_size (fst p) + compile_size l.
+Proof.
+  reflexivity.
+Qed.
+
+Lemma compile_size_app l1 l2:
+  compile_size (l1 ++ l2) = compile_size l1 + compile_size l2.
+Proof.
+  induction l1; simpl; auto.
+  rewrite !compile_size_cons. lia.
+Qed.
+
+Lemma compile_size_concat l:
+  compile_size (concat l) = sum (map compile_size l).
+Proof.
+  induction l; simpl; auto.
+  rewrite compile_size_app. lia.
+Qed.
+
+Print simplify_single.
+Print simplify_aux.
+
+Lemma pat_list_size_nil: pat_list_size nil = 0.
+Proof. reflexivity. Qed.
+
+(*TODO: unify these*)
+Lemma pat_list_size_app l1 l2:
+  pat_list_size (l1 ++ l2) = pat_list_size l1 + pat_list_size l2.
+Proof.
+  induction l1; simpl; auto. rewrite !pat_list_size_cons. lia.
+Qed.
+
+Lemma simplify_aux_smaller t a p:
+  pat_list_size (map fst (simplify_aux t a p)) <= pat_size p.
+Proof.
+  revert a.
+  induction p; simpl; intros a; try reflexivity.
+  - rewrite pat_list_size_cons, pat_list_size_nil; simpl; lia.
+  - rewrite map_app, pat_list_size_app. specialize (IHp1 a); specialize (IHp2 a).  lia.
+  - specialize (IHp (mk_let v t a)). lia.
+Qed.
+
+(*The point is that even when we split, this is all a part of the original
+  However, the pattern can indeed get bigger
+  example (simple): (Pvar x | Pvar y) :: Pwild becomes (Pvar x :: Pwild), (Pvar y :: Pwild) - 
+    the size is clearly larger
+  maybe instead we want the maximum? but that doesn't work either
+  if we did maximum, let's see
+  but by the dispatch, it should work?*)
+Print dispatch1.
+
+Lemma compile_size_nil: compile_size nil = 0.
+Proof. reflexivity. Qed.
+
+(*Another compile measures*)
+Definition iter_mult (l: list nat) : nat :=
+  fold_right mult 1 l.
+Definition pattern_list_size' (ps: list pattern) : nat :=
+  iter_mult (map (fun p => 2 ^ (pat_size p)) ps).
+Check compile_size.
+Print compile_size.
+Definition compile_size' (l: list (list pattern * A)) : nat :=
+  sum (map pattern_list_size' (map fst l)).
+
+Lemma compile_size_cons' a l:
+  compile_size' (a :: l) = pattern_list_size' (fst a) + compile_size' l.
+Proof.
+  reflexivity. Qed.
+Lemma compile_size_nil': compile_size' nil = 0.
+Proof. reflexivity. Qed.
+
+Lemma pattern_list_size_cons' p l:
+  pattern_list_size' (p :: l) = 2 ^ (pat_size p) * (pattern_list_size' l).
+Proof. reflexivity. Qed.
+Search (( ?x + ?y) * ?z).
+Search (?x ^ (?y + ?z)).
+Search (?x + ?y <= ?w + ?v).
+ Search (?x <= ?y * ?x).
+Search (?x <= ?y ^ ?z).
+
+Lemma pow_geq_1 n m:
+  n <> 0 ->
+  1 <= n ^ m.
+Proof.
+  induction m; simpl; lia.
+Qed.
+
+Lemma mul_le n m:
+  1 <= m ->
+  n <= m * n.
+Proof.
+pose proof (Arith_prebase.mult_O_le_stt n m). lia.
+Qed. 
+
+Lemma dispatch_smaller t types a rl:
+  compile_size' (snd (dispatch t types a rl)) <= compile_size' (a :: (snd rl)).
+Proof.
+  apply dispatch_elim; intros; simpl.
+  - rewrite compile_size_nil'; lia.
+  - rewrite !compile_size_cons'; simpl. rewrite pattern_list_size_cons'.
+    simpl. lia.
+  - rewrite compile_size_cons'; simpl. lia.
+  - rewrite !compile_size_cons'; simpl. 
+    rewrite pattern_list_size_cons'. simpl. lia.
+  - simpl in *. revert H H0. rewrite !compile_size_cons'; simpl.
+    rewrite !pattern_list_size_cons'; simpl. 
+    intros Hlt1 Hlt2. eapply Nat.le_trans. apply Hlt2.
+    apply (Nat.add_le_mono_l _ _ (2 ^ pat_size p * pattern_list_size' pl)) in Hlt1.
+    eapply Nat.le_trans. apply Hlt1. clear.
+    (*Why we needed exponents*)
+    rewrite Nat.add_0_r. rewrite !Nat.add_assoc. apply Nat.add_le_mono_r.
+    rewrite Nat.mul_add_distr_r, !Nat.pow_add_r.
+    apply Nat.add_le_mono.
+    + rewrite <- (Nat.mul_comm (2^ (pat_size q))). rewrite <- Nat.mul_assoc. apply mul_le, pow_geq_1. auto.
+    + rewrite <- Nat.mul_assoc. apply mul_le, pow_geq_1. auto.
+  - rewrite !compile_size_cons' in H |- *. simpl in *. rewrite pattern_list_size_cons' in H |- *; simpl in *.
+    eapply Nat.le_trans. apply H. rewrite Nat.add_0_r. nia.
+Qed.
+
+(*START: use this metric, prove the full result (maybe use simplify but prob not)*)
+      
+
+
+ assert (1 <= pat_size q) by admit. nia. lia.
+    
+    
+    
+    Search "distr". 
+
+ nia.
+
+    Search (?z + ?x <= ?z + ?y).
+    assert (Hlt3: 2 ^ pat_size p * pattern_list_size' pl +
+      
+2 ^ pat_size p * pattern_list_size' pl +
+
+ nia.
+
+
+
+ nia. lia.
+   lia.
+    nia.
+
+ lia. 
+
+ lia.
+
+Lemma dispatch_smaller t types a rl:
+  compile_size (snd (dispatch t types a rl)) <= compile_size (a :: (snd rl)).
+Proof.
+apply dispatch_elim.
+- intros. simpl. rewrite compile_size_nil; auto. lia.
+- intros. simpl. rewrite !compile_size_cons. simpl. unfold pat_list_size. lia.
+- intros. simpl. rewrite compile_size_cons. simpl. lia.
+- intros; simpl. rewrite !compile_size_cons. simpl. unfold pat_list_size; lia.
+- intros; simpl. rewrite !compile_size_cons; simpl in *.
+  rewrite !compile_size_cons in H, H0. simpl in *.
+  rewrite !pat_list_size_cons in H, H0; simpl in *.
+  (*Doesn't work: "or" becomes larger
+    So what is the termination metric? - maybe it is the 
+
+    is it possible to not terminate?
+
+    so if we have (p1 | p2) ; Pwild, end up with
+      (p1 :: Pwild), (p2 :: Pwild)
+
+    what if we do exponentially decreasing:
+    like sum (2 ^ size p) (or mult?)
+    2 ^ (|p1| + |p2| + 1) = 2 * 2^(|p1|) * 2 ^(|p2|)
+    which is larger than  2^(|p1|) * 2^(|p2|)
+
+    so this should work
+    and same for the terms
+
+    will be more complicated
+
+    like: 2^(length l) * 1 + ...
+    would be smaller if this is smaller
+    otherwise, Por = |p1| + |p2| + 1, so
+
+
+ lia.
+
+ lia.
+  
+
+ lia. 
+
+ rewrite compile_size_cons. simpl. rewrite compile_size_nil.
+Search dispatch.
+Admitted.
+
+
+Lemma dispath1_smaller t types rl:
+  compile_size (snd (dispatch1 t types rl)) <= compile_size rl.
+Proof.
+  induction rl; simpl; auto.
+
+
+  
+
+  Print dispatch1.
+
+Lemma simplify_single_smaller t ps a:
+  compile_size (simplify_single t (ps, a)) <= pat_list_size ps.
+Proof.
+  unfold simplify_single.
+  destruct ps; auto.
+  rewrite pat_list_size_cons.
+  assert (forall rl, compile_size (map (fun '(p1, y) => (p1 :: ps, y)) rl) =
+    pat_list_size (map fst rl) + pat_list_size ps).
+  {
+    intros rl. induction rl; simpl.
+
+
+  Print simplify_single.
+  revert a.
+  induction ps as [|phd ptl IH]; intros a; simpl; auto.
+  rewrite pat_list_size_cons.
+  destruct phd; simpl.
+  - rewrite compile_size_cons; simpl. unfold compile_size; simpl.
+  Search pat_list_size.
+  Print simplify_single.
+
+Lemma simplify_smaller t rl : compile_size (simplify t rl) <= compile_size rl.
+Proof.
+  unfold simplify.
+  induction rl; simpl; try lia.
+  rewrite compile_size_app, compile_size_cons.
+  (*TODO: lemma?*)
+  assert (hhd: compile_size (simplify_single t a) <= pat_list_size (fst a)).
+  {
+    destruct a as [ps a]; simpl in *.
+    destruct ps as [| phd ptl]; simpl; auto.
+    
+    unfold simplify_aux.
+    simpl.
+
+
+  unfold simplify_single. destruct a as [ps a]; simpl in *.
+  destruct ps as 
+  Print simplify_single.
+  simpl.
+
+
+  rewrite compile_size_concat.
+  induction rl; simpl; try lia.
+  rewrite compile_
+
+Lemma wild_smaller t types rl: compile_size (snd (dispatch2 t types rl)) < compile_size rl.
+Proof.
+  unfold dispatch2. Check simplify t rl.
+
+
+(*Let's try this*)
+Definition dep_let (A: Type) (x: A) : {y: A | y = x} := exist _ x eq_refl.
+Obligation Tactic := idtac.
+(*NOTE: will try to do with pattern, I think that is terminating*)
+Equations compile (tl: list (term * vty)) (rl: list (list pattern * A)) : option A 
+  by wf (compile_size rl) lt :=
+  compile _ [] := None;
+  compile [] ((_, a) :: _) => Some a;
+  compile ((t, ty) :: tl) rl =>
+    (*No bare*)
+    (*extract the set of constructors*)
+    let css :=
+    match ty with
+    | vty_cons ts _ => get_constructors ts
+    | _ => nil
+    end in
+    (*NOTE: no metadata in funsym saying constructor*)
+    let is_constr fs := in_bool funsym_eq_dec fs css in
+
+    (*Here, we do the simplify/dispatch*)
+
+    (*Map every constructor ocurring at the head of the pattern list to the
+      list of its args*)
+    let types_cslist :=
+      (*NOTE: we don't have maps, not ideal*)
+      fold_left (populate is_constr) (map (fun x => List.hd Pwild (fst x)) rl) (amap_empty, nil) 
     in 
+    let types := fst types_cslist in
+    let cslist := snd types_cslist in
     
     (*dispatch part*)
-    let (cases, wilds) := dispatch1 t types rl in
+    let casewild := dispatch1 t types rl in
+    let cases := fst casewild in
+    let wilds := snd casewild in
+    (* let (cases, wilds) := proj1_sig casewild in *)
 
-    let comp_cases cs (al : list (term * vty)) :=
+    (*let comp_cases cs (al : list (term * vty)) :=
       let l := match (amap_get funsym_eq_dec cases cs ) with
       | None => nil (*impossible*)
       | Some l => l
       end in
-      compile (rev al ++ tl) l in
+      compile (rev al ++ tl) l in*)
 
-    let comp_wilds (_: unit) := compile tl wilds in 
+    let comp_wilds (_: unit) := compile tl wilds in
 
     (*TODO: default case here*)
     let comp_full (_: unit) :=
       let no_wilds := forallb (fun f => amap_mem funsym_eq_dec f types) css in
       let base : option (list (pattern * A)) := if no_wilds then Some nil else (*TODO: bind*)
-       match comp_wilds tt with
+       match compile tl wilds with
         | None => None
         | Some x => Some [(Pwild, x)]
       end in
@@ -256,6 +722,12 @@ Equations compile (tl: list (term * vty)) (rl: list (list pattern * A)) : option
           (fst v, ty)) (combine new_var_names ql) in*)
         let pl := rev_map Pvar vl in
         let al := rev_map Tvar vl in
+        let comp_cases cs (al : list (term * vty)) :=
+          let l := match (amap_get funsym_eq_dec cases cs ) with
+          | None => nil (*impossible*)
+          | Some l => l
+          end in
+          compile (rev al ++ tl) l in
         match (comp_cases cs (combine al (map snd vl))) with
         | None => None
         | Some v => Some ((Pconstr cs params pl, v) :: acc)
@@ -276,6 +748,14 @@ Equations compile (tl: list (term * vty)) (rl: list (list pattern * A)) : option
     
     match t with
     | Tfun cs params al =>
+
+      let comp_cases cs (al : list (term * vty)) :=
+      let l := match (amap_get funsym_eq_dec cases cs ) with
+      | None => nil (*impossible*)
+      | Some l => l
+      end in
+      compile (rev al ++ tl) l in
+
       if is_constr cs then
         if amap_mem funsym_eq_dec cs types then comp_cases cs (combine al
           (map (ty_subst (s_params cs) params) (s_args cs))) else comp_wilds tt
@@ -284,9 +764,24 @@ Equations compile (tl: list (term * vty)) (rl: list (list pattern * A)) : option
       comp_full tt 
     end.
 Next Obligation.
+intros t ty tl phd ptl compile rl css is_constr types_cslist types cslist casewild cases wilds _.
+subst wilds. unfold casewild.
+rewrite dispatch_equiv.
+fold rl.
+Print dispatch2.
+Print dispatch2_gen.
+Print dispatch2_aux.
+(*TODO: prove about dispatch2*)
+
+ (*?*) compile rl css is_constr types_cslist types cslist casewild cases wilds _ no_wilds.
+set (css:= match ty with
+    | vty_cons ts _ => get_constructors ts
+    | _ => nil
+    end) in *.
 (*Problem: lose information about cases here*)
 
 (*Idea:
+  0. Prove that dispatch1/2 equivalent to filter version (will be useful for both)
   1. Prove that everything in cases has compile_size smaller than rl
   2. Prove that wilds has size smaller than rl 
   3. Probably (maybe) need to inline comp_cases/comp_wilds, or make dependently typed
